work on BtreeInv

immutable-btree/BtreeSpec.dfy
@@ -5,72 +5,130 @@ include "../lib/sequences.dfy"
 
 abstract module BtreeSpec {
   import Keyspace = Bounded_Total_Order
+  import opened Sequences
 
   type Key = Keyspace.Element
 
   datatype Node<Value> =
-    Leaf(keys: seq<Key>, values: seq<Value>) |
-    Index(pivots: seq<Key>, children: seq<Node>)
+    Leaf(keys: seq<Key>, values: seq<Value>, lb: Key, ub: Key) |
+    Index(pivots: seq<Key>, children: seq<Node>, lb: Key, ub: Key)
 
-  datatype Constants = Constants();
-  datatype Variables = Variables(root: Node);
+  datatype Constants = Constants()
+  datatype Variables<Value> = Variables(root: Node<Value>)
 
   predicate Init(k: Constants, s: Variables) {
+    s.root == Leaf([], [], Keyspace.Min_Element, Keyspace.Max_Element)
   }
 
-  datatype Layer<Value(!new)> = Layer(lb: Key, ub: Key, node: Node<Value>, slot: int)
-  type Lookup<Value(!new)> = seq<Layer<Value>>
+  predicate WFTree(tree: Node) {
+    if tree.Leaf? then
+      && |tree.keys| > 0
+      && NoDupes(tree.keys)
+      && Keyspace.IsSorted(tree.keys)
+      && |tree.keys| == |tree.values|
+      && (forall i :: 0 <= i < |tree.keys| ==> Keyspace.lte(tree.lb, tree.keys[i]) && Keyspace.lt(tree.keys[i], tree.ub))
+    else
+      && |tree.pivots| > 0
+      && Keyspace.IsSorted(tree.pivots)
+      && (forall i :: 0 <= i < |tree.pivots| ==> Keyspace.lt(tree.lb, tree.pivots[i]) && Keyspace.lt(tree.pivots[i], tree.ub))
+      && |tree.children| == |tree.pivots| + 1
+      && (forall i {:trigger WFTree(tree.children[i]) } :: 0 <= i < |tree.children| ==> WFTree(tree.children[i]))
+      && tree.lb == tree.children[0].lb
+      && tree.ub == tree.children[|tree.children| - 1].ub
+      && (forall i :: 0 <= i < |tree.pivots| ==>
+          && tree.pivots[i] == tree.children[i].ub
+          && tree.pivots[i] == tree.children[i+1].lb
+         )
+  }
 
-  predicate Get(k: Constants, s: Variables, s': Variables, key: Key, value: Value, lookup: Lookup)
+  predicate WFRoot(tree: Node) {
+    if tree.Leaf? then
+      && Keyspace.IsSorted(tree.keys)
+      && |tree.keys| == |tree.values|
+    else 
+      WFTree(tree)
+  }
+
+  datatype Layer<Value(!new)> = Layer(node: Node<Value>, slot: int)
+  type Lookup<Value(!new)> = seq<Layer<Value>>
+ 
+  predicate ValidLookup(lookup: Lookup)
+  {
+    if |lookup| == 0 then true
+    else
+      && (forall i :: 0 <= i < |lookup| - 1 ==> WFTree(lookup[i].node))
+      && (forall i :: 0 <= i < |lookup| - 1 ==> lookup[i].node.Index?)
+      && (forall i :: 0 <= i < |lookup| - 1 ==> 0 <= lookup[i].slot < |lookup[i].node.children|)
+      && (forall i :: 0 <= i < |lookup| - 1 ==> lookup[i+1].node == lookup[i].node.children[lookup[i].slot])
+      && WFTree(Last(lookup).node)
+      && Last(lookup).node.Leaf?
+      && 0 <= Last(lookup).slot < |Last(lookup).node.keys|
+  }
+
+  predicate IsSatisfyingLookup<Value(!new)>(tree: Node, key: Key, value: Value, lookup: Lookup)
+  {
+    && ValidLookup(lookup)
+    && |lookup| > 0
+    && lookup[0].node == tree
+    && Last(lookup).node.keys[Last(lookup).slot] == key 
+    && Last(lookup).node.values[Last(lookup).slot] == value
+  }
+
+  predicate Get<Value>(k: Constants, s: Variables, s': Variables, key: Key, value: Value, lookup: Lookup)
   {
     && IsSatisfyingLookup(s.root, key, value, lookup)
     && s' == s
   }
 
-  predicate PutTransform(tree:Node, newtree:Node, key:Key, value:Value)
+  predicate PutTransform<Value>(tree:Node, newtree:Node, key:Key, value:Value)
+    requires WFTree(tree)
     decreases tree;
   {
-    if tree.Leaf? then (
-      var pos := Keyspace.LargestLte(tree.keys, query);
-      if pos >= 0 && query == tree.keys[pos] (
-        newtree == Leaf(tree.keys, tree.values[pos := value]);
+    && tree.lb == newtree.lb
+    && tree.ub == newtree.ub
+    && (if tree.Leaf? then (
+      var pos := Keyspace.LargestLte(tree.keys, key);
+      if pos >= 0 && key == tree.keys[pos] then (
+        newtree == Leaf(tree.keys, tree.values[pos := value], tree.lb, tree.ub)
       ) else (
-        var newkeys := tree.keys[..pos+1] + [query] + tree.keys[pos+1..];
+        var newkeys := tree.keys[..pos+1] + [key] + tree.keys[pos+1..];
         var newvals := tree.values[..pos+1] + [value] + tree.values[pos+1..];
-        newtree == Leaf(newkeys, newvals);
+        newtree == Leaf(newkeys, newvals, tree.lb, tree.ub)
       )
     ) else (
-      var pos := Keyspace.LargestLte(tree.pivots, query) + 1;
-      var newlb := LeftBound(lb, tree.pivots, tree.children, pos);
-      var newub := RightBound(tree.pivots, tree.children, ub, pos);
+      && var pos := Keyspace.LargestLte(tree.pivots, key) + 1;
 
-      // Before we can call Define recursively, we must prove that the child CantEquivocate.
-      var newchild := PutTransform(newlb, tree.children[pos], newub, query, value);
-      newtree := Index(tree.pivots, tree.children[pos := newchild]);
-    )
+      && newtree.Index?
+      && newtree.pivots == tree.pivots
+      && |newtree.children| == |tree.children|
+      && newtree.children == tree.children[pos := newtree.children[pos]]
+      && PutTransform(tree.children[pos], newtree.children[pos], key, value)
+    ))
   }
 
-  predicate Put(k: Constants, s: Variables, s': Variables, key: Key, value: Value)
+  predicate Put<Value>(k: Constants, s: Variables, s': Variables, key: Key, value: Value)
   {
+    && WFTree(s.root)
     && PutTransform(s.root, s'.root, key, value)
   }
 
-  datatype Step =
+  datatype Step<Value(!new)> =
     | GetStep(key: Key, value: Value, lookup: Lookup)
     | PutStep(key: Key, value: Value)
-    | SplitStep()
-    | GrowStep()
+    //| SplitStep()
+    //| GrowStep()
+    /*| ContractStep()*/
 
   predicate NextStep(k: Constants, s: Variables, s': Variables, step:Step) {
     match step {
       case GetStep(key, value, lookup) => Get(k, s, s', key, value, lookup)
-      case PutStep() => Put(k, s, s', key, value)
-      case SplitStep() => Split(k, s, s')
-      case GrowStep() => GrowStep(k, s, s')
+      case PutStep(key, value) => Put(k, s, s', key, value)
+      /*case SplitStep() => Split(k, s, s')
+      case GrowStep() => GrowStep(k, s, s')*/
     }
   }
 
-  predicate Next(k: Constants, s: Variables, s': Variables) {
+  predicate Next<Value(!new)>(k: Constants, s: Variables, s': Variables) {
     exists step:Step :: NextStep(k, s, s', step)
   }
 
