immutable-btree/BtreeInv.dfy
@@ -1,0 +1,202 @@
+include "../lib/total_order.dfy"
+include "../lib/map_utils.dfy"
+include "../lib/mathematics.dfy"
+include "../lib/sequences.dfy"
+include "BtreeSpec.dfy"
+
+abstract module BtreeInv {
+  import Keyspace = Bounded_Total_Order
+  import opened Sequences
+  import opened BtreeSpec
+
+  predicate CantEquivocate<Value(!new)>(tree: Node<Value>)
+  {
+    forall key, value, value', lookup: Lookup<Value>, lookup': Lookup<Value> ::
+      && IsSatisfyingLookup(tree, key, value, lookup)
+      && IsSatisfyingLookup(tree, key, value', lookup') ==>
+      value == value'
+  }
+
+
+  predicate Invariant(k: Constants, s: Variables) {
+    && WFTree(s.root)
+    && CantEquivocate(s.root)
+  }
+
+
+  predicate PreservesLookups<Value(!new)>(tree: Node, newtree: Node)
+  {
+    forall lookup, key, value :: IsSatisfyingLookup(tree, key, value, lookup) ==>
+    exists lookup' :: IsSatisfyingLookup(newtree, key, value, lookup')
+  }
+
+  predicate PreservesLookupsExcept<Value(!new)>(tree: Node, newtree: Node, exceptQuery: Key)
+  {
+    forall lookup, key, value :: key != exceptQuery && IsSatisfyingLookup(tree, key, value, lookup) ==>
+    exists lookup' :: IsSatisfyingLookup(newtree, key, value, lookup')
+  }
+
+  lemma SatisfyingLookupsNest<Value(!new)>(tree: Node, key: Key, value: Value, lookup: Lookup)
+    requires IsSatisfyingLookup(tree, key, value, lookup);
+    requires tree.Index?;
+    ensures IsSatisfyingLookup(tree.children[lookup[0].slot],
+                               key, value,
+                               lookup[1..]);
+  {
+  }
+
+  lemma SatisfyingLookupSlotIsLargestLte<Value>(tree: Node, key: Key, value: Value, lookup: Lookup)
+    requires IsSatisfyingLookup(tree, key, value, lookup);
+    requires tree.Index?;
+    ensures lookup[0].slot == Keyspace.LargestLte(tree.pivots, key) + 1;
+  {
+    var pos := Keyspace.LargestLte(tree.pivots, key) + 1;
+    if lookup[0].slot < pos {
+      SatisfyingLookupsNest(tree, key, value, lookup);
+      assert Keyspace.lt(key, lookup[1].node.ub);
+      assert Keyspace.lte(lookup[1].node.ub, tree.pivots[lookup[0].slot]);
+      assert Keyspace.lte(tree.pivots[lookup[0].slot], tree.pivots[pos-1]);
+      assert Keyspace.lte(tree.pivots[pos-1], key);
+      assert false;
+    } else if lookup[0].slot > pos {
+      SatisfyingLookupsNest(tree, key, value, lookup);
+      assert Keyspace.lt(key, tree.pivots[pos]);
+      assert Keyspace.lte(tree.pivots[pos], tree.pivots[lookup[0].slot-1]);
+      assert Keyspace.lte(tree.pivots[lookup[0].slot-1], lookup[1].node.lb);
+      assert Keyspace.lte(lookup[1].node.lb, key);
+      assert false;
+    }
+  }
+
+  lemma PutIsCorrect<Value>(tree: Node, newtree: Node, key: Key, value: Value)
+  requires WFTree(tree)
+  requires CantEquivocate(tree)
+  requires PutTransform(tree, newtree, key, value);
+  ensures PreservesLookupsExcept(tree, newtree, key);
+  ensures PreservesLookupsExcept(newtree, tree, key);
+  ensures exists lookup :: IsSatisfyingLookup(newtree, key, value, lookup);
+  ensures CantEquivocate(newtree)
+  decreases tree
+  {
+    reveal_NoDupes();
+    if tree.Leaf? {
+      var pos := Keyspace.LargestLte(tree.keys, key);
+      if pos >= 0 && key == tree.keys[pos] {
+        assert newtree == Leaf(tree.keys, tree.values[pos := value], tree.lb, tree.ub);
+        
+        forall lookup: Lookup, key', value'
+          | key' != key && IsSatisfyingLookup(tree, key', value', lookup)
+          ensures exists lookup' :: IsSatisfyingLookup(newtree, key', value', lookup');
+        {
+          var lookup' := [Layer(newtree, lookup[0].slot)];
+          assert IsSatisfyingLookup(newtree, key', value', lookup');
+        }
+        forall lookup': Lookup, key', value'
+          | key' != key && IsSatisfyingLookup(newtree, key', value', lookup')
+          ensures exists lookup :: IsSatisfyingLookup(tree, key', value', lookup);
+        {
+          var lookup := [Layer(tree, lookup'[0].slot)];
+          assert IsSatisfyingLookup(tree, key', value', lookup);
+        }
+
+        assert IsSatisfyingLookup(newtree, key, value, [Layer(newtree, pos)]);
+
+      } else {
+        var newkeys := tree.keys[..pos+1] + [key] + tree.keys[pos+1..];
+        var newvals := tree.values[..pos+1] + [value] + tree.values[pos+1..];
+        assert newtree == Leaf(newkeys, newvals, tree.lb, tree.ub);
+        //assert Keyspace.IsSorted(newtree.keys);
+        assert IsSatisfyingLookup(newtree, key, value, [Layer(newtree, pos + 1)]);
+        
+        forall lookup: Lookup, key', value'
+          | key' != key && IsSatisfyingLookup(tree, key', value', lookup)
+          ensures exists lookup' :: IsSatisfyingLookup(newtree, key', value', lookup');
+        {
+          if lookup[0].slot <= pos {
+            var lookup' := [Layer(newtree, lookup[0].slot)];
+            assert IsSatisfyingLookup(newtree, key', value', lookup');
+          } else {
+            var lookup' := [Layer(newtree, lookup[0].slot + 1)];
+            assert IsSatisfyingLookup(newtree, key', value', lookup');
+          }
+        }
+        forall lookup': Lookup, key', value'
+          | key' != key && IsSatisfyingLookup(newtree, key', value', lookup')
+          ensures exists lookup :: IsSatisfyingLookup(tree, key', value', lookup);
+        {
+          assert lookup'[0].slot != pos+1;
+          if lookup'[0].slot <= pos {
+            var lookup := [Layer(tree, lookup'[0].slot)];
+            assert IsSatisfyingLookup(tree, key', value', lookup);
+          } else {
+            var lookup := [Layer(tree, lookup'[0].slot - 1)];
+            assert IsSatisfyingLookup(tree, key', value', lookup);
+          }
+        }
+
+      }
+    } else {
+      var pos := Keyspace.LargestLte(tree.pivots, key) + 1;
+
+      // Before we can call Define recursively, we must prove that the child CantEquivocate.
+      forall key', valueA, valueB, lookup, lookup'
+      |
+      && IsSatisfyingLookup(tree.children[pos], key', valueA, lookup)
+      && IsSatisfyingLookup(tree.children[pos], key', valueB, lookup')
+      ensures valueA == valueB;
+      {
+        var plookup  := [Layer(tree, pos)] + lookup;
+        var plookup' := [Layer(tree, pos)] + lookup';
+        assert IsSatisfyingLookup(tree, key', valueA, plookup);
+        assert IsSatisfyingLookup(tree, key', valueB, plookup');
+      }
+      var newchild := newtree.children[pos];
+      PutIsCorrect(tree.children[pos], newchild, key, value);
+      assert PutTransform(tree.children[pos], newchild, key, value);
+      assert newtree == Index(tree.pivots, tree.children[pos := newchild], tree.lb, tree.ub);
+
+      // PreservesLookupsExcept proofs
+      forall lookup: Lookup, key', value'
+        | key' != key && IsSatisfyingLookup(tree, key', value', lookup)
+        ensures exists lookup' :: IsSatisfyingLookup(newtree, key', value', lookup');
+      {
+        SatisfyingLookupsNest(tree, key', value', lookup);
+        var clookup := lookup[1..];
+        assert IsSatisfyingLookup(tree.children[lookup[0].slot], key', value', clookup);
+        var clookup' :| IsSatisfyingLookup(newtree.children[lookup[0].slot], key', value', clookup');
+        var lookup' := [Layer(newtree, lookup[0].slot)] + clookup';
+        assert IsSatisfyingLookup(newtree, key', value', lookup');
+      }
+      forall lookup': Lookup, key', value'
+        | key' != key && IsSatisfyingLookup(newtree, key', value', lookup')
+        ensures exists lookup :: IsSatisfyingLookup(tree, key', value', lookup);
+      {
+        SatisfyingLookupsNest(newtree, key', value', lookup');
+        var clookup' := lookup'[1..];
+        assert IsSatisfyingLookup(newtree.children[lookup'[0].slot], key', value', clookup');
+        var clookup: Lookup<Value> :| IsSatisfyingLookup(tree.children[lookup'[0].slot], key', value', clookup);
+        var lookup := [Layer(tree, lookup'[0].slot)] + clookup;
+        assert IsSatisfyingLookup(tree, key', value', lookup);
+      }
+
+      // Proof that we can lookup key and get value
+      ghost var clookup :| IsSatisfyingLookup(newtree.children[pos], key, value, clookup);
+      ghost var lookup := [Layer(newtree, pos)] + clookup;
+      assert IsSatisfyingLookup(newtree, key, value, lookup);
+
+      // Proof that we CantEquivocate
+      forall key', valueA, valueB, lookupA: Lookup, lookupB: Lookup
+      |
+      && IsSatisfyingLookup(newtree, key', valueA, lookupA)
+      && IsSatisfyingLookup(newtree, key', valueB, lookupB)
+      ensures valueA == valueB;
+      {
+        SatisfyingLookupSlotIsLargestLte(newtree, key', valueA, lookupA);
+        SatisfyingLookupSlotIsLargestLte(newtree, key', valueB, lookupB);
+        SatisfyingLookupsNest(newtree, key', valueA, lookupA);
+        SatisfyingLookupsNest(newtree, key', valueB, lookupB);
+      }
+      assert CantEquivocate(newtree);
+    }
+  }
+}
